Instances/ISAs/VexSummary.lean
@@ -12,6 +12,7 @@ inductive SymExpr (Reg : Type) where
   | reg : Reg → SymExpr Reg
   | low32 : SymExpr Reg → SymExpr Reg
   | uext32 : SymExpr Reg → SymExpr Reg
+  | sext8to32 : SymExpr Reg → SymExpr Reg
   | add64 : SymExpr Reg → SymExpr Reg → SymExpr Reg
   | sub64 : SymExpr Reg → SymExpr Reg → SymExpr Reg
   | xor64 : SymExpr Reg → SymExpr Reg → SymExpr Reg
@@ -129,6 +130,7 @@ mutual
   | .reg reg => state.read reg
   | .low32 expr => mask32 (evalSymExpr state expr)
   | .uext32 expr => mask32 (evalSymExpr state expr)
+  | .sext8to32 expr => signExtend8to32 (evalSymExpr state expr)
   | .add64 lhs rhs => evalSymExpr state lhs + evalSymExpr state rhs
   | .sub64 lhs rhs => evalSymExpr state lhs - evalSymExpr state rhs
   | .xor64 lhs rhs => evalSymExpr state lhs ^^^ evalSymExpr state rhs
@@ -166,6 +168,7 @@ def substSymExpr {Reg : Type} [DecidableEq Reg] [Fintype Reg]
   | .reg reg => sub.regs reg
   | .low32 expr => .low32 (substSymExpr sub expr)
   | .uext32 expr => .uext32 (substSymExpr sub expr)
+  | .sext8to32 expr => .sext8to32 (substSymExpr sub expr)
   | .add64 lhs rhs => .add64 (substSymExpr sub lhs) (substSymExpr sub rhs)
   | .sub64 lhs rhs => .sub64 (substSymExpr sub lhs) (substSymExpr sub rhs)
   | .xor64 lhs rhs => .xor64 (substSymExpr sub lhs) (substSymExpr sub rhs)
@@ -250,6 +253,7 @@ theorem substSymExpr_id {Reg : Type} [DecidableEq Reg] [Fintype Reg] (expr : Sym
   | reg reg => rfl
   | low32 expr => simp [substSymExpr, substSymExpr_id]
   | uext32 expr => simp [substSymExpr, substSymExpr_id]
+  | sext8to32 expr => simp [substSymExpr, substSymExpr_id]
   | add64 lhs rhs =>
       simp [substSymExpr, substSymExpr_id]
   | sub64 lhs rhs =>
@@ -284,6 +288,7 @@ theorem substSymExpr_compose {Reg : Type} [DecidableEq Reg] [Fintype Reg]
   | reg reg => rfl
   | low32 expr => simp [substSymExpr, substSymExpr_compose]
   | uext32 expr => simp [substSymExpr, substSymExpr_compose]
+  | sext8to32 expr => simp [substSymExpr, substSymExpr_compose]
   | add64 lhs rhs =>
       simp [substSymExpr, substSymExpr_compose]
   | sub64 lhs rhs =>
@@ -319,6 +324,7 @@ theorem evalSymExpr_subst {Reg : Type} [DecidableEq Reg] [Fintype Reg]
   | reg reg => rfl
   | low32 expr => simp [substSymExpr, evalSymExpr_subst]
   | uext32 expr => simp [substSymExpr, evalSymExpr_subst]
+  | sext8to32 expr => simp [substSymExpr, evalSymExpr_subst]
   | add64 lhs rhs =>
       simp [substSymExpr, evalSymExpr_subst]
   | sub64 lhs rhs =>
